create solution stubs and prove ending cases with attending lemmas

leetcode/preorderTraversal.dfy
@@ -32,6 +32,15 @@ module PreorderTraversal {
         (if node.right != null then {node.right} else {}) + 
         (if node.left != null then {node.left} else {})
     }
+
+    lemma childrenLemma(node: TreeNode)
+        requires node.Valid()
+        ensures children(node) < node.repr
+        ensures node !in children(node)
+    {
+
+    }
+
     function childStack(node: TreeNode?): seq<TreeNode> 
         reads if node == null then {} else node.repr
         requires node != null ==> node.Valid()
@@ -138,6 +147,26 @@ module PreorderTraversal {
       ensures AllAncestors(pruneParents(ss, visited))
     {
 
+    }
+
+    lemma pruneParentsLemma2(ss: seq<TreeNode>, visited: set<TreeNode>)
+      requires AllAncestors(ss)
+      requires ss!=[]
+      requires pruneParents(ss, visited) == []
+      ensures forall x: TreeNode :: x in ss && x !in pruneParents(ss, visited) ==> children(x) <= visited
+    {
+      if ss == [] {
+
+      }else if |ss| == 1 {
+        assert ss[0] in ss;
+        if children(ss[0])<= visited {
+          assert ss[0] !in  pruneParents(ss, visited);
+        }else{
+          assert ss[0] in  pruneParents(ss, visited);
+        }
+      }else{
+
+      }
     }
 
   predicate compare(a: TreeNode, b: TreeNode)
@@ -317,7 +346,119 @@ lemma ThereIsAMinimum(s: set<TreeNode>)
         }
     }
 
-    lemma {:verify false} {:vcs_split_on_every_assert} traverseMaint(
+    lemma FlatMapVisitedARN(stack: seq<TreeNode>, parents: seq<TreeNode>, visited: set<TreeNode>, current: TreeNode)
+      requires |stack| > 0 
+      requires current == stack[|stack|-1]
+      requires current !in visited
+      requires current.Valid()
+      requires stack == Seq.Flatten(Seq.Map((x: TreeNode) reads x => rightStackVisited(x, visited), parents))
+      ensures stack[..|stack|-1] == allRight(pruneParents(parents+parentStack(current), visited+{current}), visited+{current})
+    {
+    }
+
+    lemma FlatMapVisitedARL(stack: seq<TreeNode>, parents: seq<TreeNode>, visited: set<TreeNode>, current: TreeNode, newStack: seq<TreeNode>, newParents: seq<TreeNode>)
+      requires |stack| > 0 
+      requires current == stack[|stack|-1]
+      requires current !in visited
+      requires current.Valid()
+      requires forall parent :: parent in parents ==> parent.Valid()
+      requires stack == allRight(parents, visited)
+      requires newParents == pruneParents(parents+parentStack(stack[|stack|-1]), visited+{stack[|stack|-1]})
+      requires newStack == stack[..|stack|-1] + childStack(stack[ |stack|-1])
+      requires childStack(current) == [current.left]
+      ensures stackPred2(newStack, newParents, visited+{current})
+    {
+    }
+
+    lemma FlatMapVisitedARR(stack: seq<TreeNode>, parents: seq<TreeNode>, visited: set<TreeNode>, current: TreeNode, newStack: seq<TreeNode>, newParents: seq<TreeNode>)
+      requires |stack| > 0 
+      requires current == stack[|stack|-1]
+      requires current !in visited
+      requires current.Valid()
+      requires forall parent :: parent in parents ==> parent.Valid()
+      requires stack == allRight(parents, visited)
+      requires newParents == pruneParents(parents+parentStack(stack[|stack|-1]), visited+{stack[|stack|-1]})
+      requires newStack == stack[..|stack|-1] + childStack(stack[ |stack|-1])
+      requires childStack(current) == [current.right]
+      ensures stackPred2(newStack, newParents, visited+{current})
+    {
+    }
+
+    lemma FlatMapVisitedARBoth(stack: seq<TreeNode>, parents: seq<TreeNode>, visited: set<TreeNode>, current: TreeNode, newStack: seq<TreeNode>, newParents: seq<TreeNode>)
+      requires |stack| > 0 
+      requires current == stack[|stack|-1]
+      requires current !in visited
+      requires current.Valid()
+      requires forall parent :: parent in parents ==> parent.Valid()
+      requires stack == allRight(parents, visited)
+      requires newParents == pruneParents(parents+parentStack(stack[|stack|-1]), visited+{stack[|stack|-1]})
+      requires newStack == stack[..|stack|-1] + childStack(stack[ |stack|-1])
+      requires childStack(current) == [current.right, current.left]
+      ensures stackPred2(newStack, newParents, visited+{current})
+    {
+    }
+
+    lemma FlatMapVisitedPCN(stack: seq<TreeNode>, parents: seq<TreeNode>, visited: set<TreeNode>, current: TreeNode, newStack: seq<TreeNode>, newParents: seq<TreeNode>)
+      requires |stack| > 0 
+      requires current == stack[|stack|-1]
+      requires current !in visited
+      requires current.Valid()
+      requires parents != []
+      requires forall parent :: parent in parents ==> parent.Valid()
+      requires stack == allRightPlusChildren(parents, visited)
+      requires newParents == pruneParents(parents+parentStack(stack[|stack|-1]), visited+{stack[|stack|-1]})
+      requires newStack == stack[..|stack|-1] + childStack(stack[ |stack|-1])
+      requires childStack(current) == []
+      ensures stackPred2(newStack, newParents, visited+{current})
+    {
+    }
+
+    lemma FlatMapVisitedPCL(stack: seq<TreeNode>, parents: seq<TreeNode>, visited: set<TreeNode>, current: TreeNode, newStack: seq<TreeNode>, newParents: seq<TreeNode>)
+      requires |stack| > 0 
+      requires current == stack[|stack|-1]
+      requires current !in visited
+      requires current.Valid()
+      requires parents != []
+      requires forall parent :: parent in parents ==> parent.Valid()
+      requires stack == allRightPlusChildren(parents, visited)
+      requires newParents == pruneParents(parents+parentStack(stack[|stack|-1]), visited+{stack[|stack|-1]})
+      requires newStack == stack[..|stack|-1] + childStack(stack[ |stack|-1])
+      requires childStack(current) == [current.left]
+      ensures stackPred2(newStack, newParents, visited+{current})
+    {
+    }
+
+    lemma FlatMapVisitedPCR(stack: seq<TreeNode>, parents: seq<TreeNode>, visited: set<TreeNode>, current: TreeNode, newStack: seq<TreeNode>, newParents: seq<TreeNode>)
+      requires |stack| > 0 
+      requires current == stack[|stack|-1]
+      requires current !in visited
+      requires current.Valid()
+      requires parents != []
+      requires forall parent :: parent in parents ==> parent.Valid()
+      requires stack == allRightPlusChildren(parents, visited)
+      requires newParents == pruneParents(parents+parentStack(stack[|stack|-1]), visited+{stack[|stack|-1]})
+      requires newStack == stack[..|stack|-1] + childStack(stack[ |stack|-1])
+      requires childStack(current) == [current.right]
+      ensures stackPred2(newStack, newParents, visited+{current})
+    {
+    }
+
+    lemma FlatMapVisitedPCBoth(stack: seq<TreeNode>, parents: seq<TreeNode>, visited: set<TreeNode>, current: TreeNode, newStack: seq<TreeNode>, newParents: seq<TreeNode>)
+      requires |stack| > 0 
+      requires current == stack[|stack|-1]
+      requires current !in visited
+      requires current.Valid()
+      requires parents != []
+      requires forall parent :: parent in parents ==> parent.Valid()
+      requires stack == allRightPlusChildren(parents, visited)
+      requires newParents == pruneParents(parents+parentStack(stack[|stack|-1]), visited+{stack[|stack|-1]})
+      requires newStack == stack[..|stack|-1] + childStack(stack[ |stack|-1])
+      requires childStack(current) == [current.right, current.left]
+      ensures stackPred2(newStack, newParents, visited+{current})
+    {
+    }
+
+    lemma {:verify } {:vcs_split_on_every_assert} traverseMaint(
         root: TreeNode,
         result: seq<TreeNode>,
         visited: set<TreeNode>,
@@ -338,18 +479,17 @@ lemma ThereIsAMinimum(s: set<TreeNode>)
       requires parents != [] ==> stackPred2(stack, parents, visited)
       requires unvisited !! visited
       requires unvisited + visited == root.repr
-      // requires visited <= root.repr
-      // requires |visited| <= |root.repr|
       requires forall x :: x in stack ==> x in unvisited
       requires AllDisjoint(stack)
       requires unvisited == TreeUnion(stack)
       // requires i == |result|
-      // requires i == |visited|
       // requires 0 <= i <= |PreorderTraversal(root)|
       // requires result == PreorderTraversal(root)[..i]
       // requires |stack| > 0 && i < |PreorderTraversal(root)| ==> stack[|stack|-1] == PreorderTraversal(root)[i]
       ensures AllAncestors(pruneParents(parents+parentStack(stack[|stack|-1]), visited+{stack[|stack|-1]}))
       ensures forall x :: x in pruneParents(parents+parentStack(stack[|stack|-1]), visited+{stack[|stack|-1]}) ==> x.Valid()
+      ensures parents != [] && pruneParents(parents+parentStack(stack[|stack|-1]), visited+{stack[|stack|-1]}) != [] ==> stackPred2(stack[..|stack|-1]+childStack(stack[|stack|-1]), pruneParents(parents+parentStack(stack[|stack|-1]), visited+{stack[|stack|-1]}), visited+{stack[|stack|-1]})
+      ensures parents != [] && pruneParents(parents+parentStack(stack[|stack|-1]), visited+{stack[|stack|-1]}) == [] ==> stack[..|stack|-1]+childStack(stack[|stack|-1]) == []
       // ensures stack[..|stack|-1]+childStack(stack[|stack|-1]) == 
     {
       assert forall x :: x in parents+parentStack(stack[|stack|-1]) ==> x.Valid() by {
@@ -377,22 +517,106 @@ lemma ThereIsAMinimum(s: set<TreeNode>)
         assert AllAncestors(parents+parentStack(stack[|stack|-1]));
         pruneParentsLemma(parents+parentStack(stack[|stack|-1]), visited+{stack[|stack|-1]});
       }
-      var newParents := pruneParents(parents, visited+{stack[|stack|-1]})+parentStack(stack[|stack|-1]);
+      var newParents := pruneParents(parents+parentStack(stack[|stack|-1]), visited+{stack[|stack|-1]});
       var newStack := stack[..|stack|-1]+childStack(stack[|stack|-1]);
-      if newParents != [] && parents != [] {
+      var current := stack[|stack|-1];
+      if parents != [] {
+      if newParents != []  {
         if |childStack(stack[|stack|-1])| > 0 {
           assert parentStack(stack[|stack|-1]) == [stack[|stack|-1]];
         }else{
           assert parentStack(stack[|stack|-1]) == [];
         }
         // assert childOf(newStack[|newStack|-1], newParents[|newParents|-1]);
-        assert stackPred2(newStack, newParents, visited+{stack[|stack|-1]}) by {
-          if stack == Seq.Flatten(Seq.Map(rightStack, parents)) {
+        assert stackPred2(newStack, newParents, visited+{current}) by {
+          childStackLemma(current);
+          var visitMap := (x: TreeNode) reads x => rightStackVisited(x, visited);
+          var newVisitMap := (x: TreeNode) reads x => rightStackVisited(x, visited+{current});
+          if stack == allRight(parents, visited) {
+            if childStack(current) == [current.right, current.left] {
+              FlatMapVisitedARBoth(stack, parents, visited, current, newStack, newParents);
+            }else if  childStack(current) == [current.left] {
+              FlatMapVisitedARL(stack, parents, visited, current, newStack, newParents);
 
-          }else if stack == Seq.Flatten(Seq.Map(rightStack, parents[..|parents|-1]))+childStack(parents[|parents|-1]) {
-
+            }else if childStack(current) == [current.right] {
+              FlatMapVisitedARR(stack, parents, visited, current, newStack, newParents);
+            }else if childStack(current) == [] {
+              FlatMapVisitedARN(stack, parents, visited, current);
+              assert newStack == Seq.Flatten(Seq.Map(newVisitMap, newParents));
+              assert stackPred2(newStack, newParents, visited+{current});
+            }
+          }else if |parents| > 0 && stack == allRightPlusChildren(parents, visited) {
+            if childStack(current) == [current.right, current.left] {
+              FlatMapVisitedPCBoth(stack, parents, visited, current, newStack, newParents);
+            }else if  childStack(current) == [current.left] {
+              FlatMapVisitedPCL(stack, parents, visited, current, newStack, newParents);
+            }else if childStack(current) == [current.right] {
+              FlatMapVisitedPCR(stack, parents, visited, current, newStack, newParents);
+            }else if childStack(current) == [] {
+              FlatMapVisitedPCN(stack, parents, visited, current, newStack, newParents);
+            }
           }
         }
+      }
+      }
+
+      if parents != [] && pruneParents(parents+parentStack(stack[|stack|-1]), visited+{stack[|stack|-1]}) == [] {
+        // assert TreeUnion(stack[|stack|-1]);
+        pruneParentsLemma2(parents+parentStack(stack[|stack|-1]), visited+{stack[|stack|-1]});
+        assert forall x :: x in parents+parentStack(stack[|stack|-1]) ==> children(x) <= visited+{current};
+        if parentStack(stack[|stack|-1]) != [] {
+          assert children(current) <= visited+{current};
+          TreeUnionLemma(stack);
+          // assert forall x :: x in children(current) ==> x in current.repr && x in unvisited && x !in visited+{current};
+          childrenLemma(current);
+          // assert forall x :: x in children(current) ==> x in current.repr && x in unvisited;
+          assert forall x :: x in children(current) ==> x in current.repr;
+          assert forall x :: x in children(current) ==> x in unvisited by {
+            forall x | x in children(current)
+              ensures x in unvisited
+            {
+              TreeUnionLemma2(stack, current, x);
+            }
+          }
+          assert false;
+        }
+        assert parents+parentStack(stack[|stack|-1])  == parents;
+        // assert visited+{stack[|stack|-1]} == root.repr;
+        assert childStack(stack[|stack|-1]) == [];
+        assert stack[..|stack|-1] == [] by {
+          if stack[..|stack|-1] != [] {
+            if stack == allRight(parents, visited) {
+              allRightLemma(parents, visited);
+              assert stack == stack[..|stack|-1]+[current];
+              forall x | x in stack 
+                ensures x in visited+{current}
+              {
+                var i :| 0 <= i < |parents| && x in rightStackVisited(parents[i], visited);
+                assert x in children(parents[i]);
+                assert parents[i] in parents;
+                assert children(parents[i]) <= visited + {current};
+              }
+              assert visited !! unvisited;
+              forall x | x in stack[..|stack|-1] 
+                ensures x in visited
+              {
+                assert x in stack;
+                assert x in unvisited;
+                assert x in visited;
+
+              }
+              var somex :| somex in stack[..|stack|-1];
+              assert somex in visited;
+              assert false;
+            } else if stack == allRightPlusChildren(parents, visited) {
+              allRightPlusChildrenLemma(parents, visited);
+              var somex :| somex in stack[..|stack|-1];
+              assert somex in visited;
+              assert false;
+            }
+          }
+        }
+        assert stack[..|stack|-1]+childStack(stack[|stack|-1]) == [];
       }
     }
 
@@ -403,12 +627,86 @@ lemma ThereIsAMinimum(s: set<TreeNode>)
       stack == Seq.Flatten(Seq.Map(rightStack, parents)) || (|parents| > 0 && stack == Seq.Flatten(Seq.Map(rightStack, parents[..|parents|-1]))+childStack(parents[|parents|-1]))
     }
 
+    function allRight(parents: seq<TreeNode>, visited: set<TreeNode>): seq<TreeNode> 
+      reads parents, set i | 0 <= i < |parents| :: parents[i], reprUnion(parents)
+    {
+      var visitMap := (x: TreeNode) reads x => rightStackVisited(x, visited);
+      Seq.Flatten(Seq.Map(visitMap, parents))
+    }
+
+    lemma flattenLemma<T>(xs: seq<seq<T>>, x: T)
+      requires x in Seq.Flatten(xs)
+      ensures x in Seq.Flatten(xs) ==> exists xx :: xx in xs && x in xx
+    {
+      if |xs| == 1 {
+        assert xs[0] in xs;
+        if x in xs[0] {
+
+        }else {
+          assert x !in xs[0];
+          assert x in Seq.Flatten(xs);
+          assert xs[1..] == [];
+          assert Seq.Flatten(xs) == xs[0];
+          assert false;
+        }
+      }else{
+        assert xs == [xs[0]] + xs[1..];
+        Seq.LemmaFlattenConcat([xs[0]], xs[1..]);
+        if x in xs[0] {
+
+        }else {
+          flattenLemma(xs[1..], x);
+        }
+
+      }
+    }
+
+    lemma allRightLemma(parents: seq<TreeNode>, visited: set<TreeNode>)
+      ensures forall x :: x in allRight(parents, visited) ==> exists i :: 0 <= i < |parents| && x in rightStackVisited(parents[i], visited)
+    {
+      forall x | x in allRight(parents, visited)
+        ensures exists i :: 0 <= i < |parents| && x in rightStackVisited(parents[i], visited)
+      {
+      var visitMap := (x: TreeNode) reads x => rightStackVisited(x, visited);
+        assert forall  k :: 0 <= k < |parents| ==> Seq.Map(visitMap, parents)[k] == rightStackVisited(parents[k], visited);
+        flattenLemma(Seq.Map(visitMap, parents), x);
+      }
+    }
+
+    function allRightPlusChildren(parents: seq<TreeNode>, visited: set<TreeNode>): seq<TreeNode>
+      reads parents, set i | 0 <= i < |parents| :: parents[i], reprUnion(parents)
+      requires |parents| > 0
+      requires forall parent :: parent in parents ==> parent.Valid()
+    {
+      var visitMap := (x: TreeNode) reads x => rightStackVisited(x, visited);
+      Seq.Flatten(Seq.Map(visitMap, parents[..|parents|-1]))+childStack(parents[|parents|-1])
+    }
+
+    lemma allRightPlusChildrenLemma(parents: seq<TreeNode>, visited: set<TreeNode>)
+      requires |parents| > 0
+      requires forall parent :: parent in parents ==> parent.Valid()
+      ensures forall x :: x in allRightPlusChildren(parents, visited) ==> exists i :: 0 <= i < |parents| && x in children(parents[i])
+    {
+      forall x | x in allRightPlusChildren(parents, visited)
+        ensures exists i :: 0 <= i < |parents| && x in children(parents[i])
+      {
+        //Seq.Flatten(Seq.Map(visitMap, parents[..|parents|-1]))+childStack(parents[|parents|-1])
+        var visitMap := (x: TreeNode) reads x => rightStackVisited(x, visited);
+        if x in Seq.Flatten(Seq.Map(visitMap, parents[..|parents|-1])) {
+        allRightLemma(parents[..|parents|-1], visited);
+        assert forall x :: x in allRight(parents[..|parents|-1], visited) ==> exists k :: 0 <= k < |parents[..|parents|-1]| && x in rightStackVisited(parents[..|parents|-1][k], visited);
+        }else{
+          assert x in childStack(parents[|parents|-1]);
+          assert x in children(parents[|parents|-1]);
+        }
+      }
+    }
+
     predicate stackPred2(stack: seq<TreeNode>, parents: seq<TreeNode>, visited: set<TreeNode>) 
       reads parents, set i | 0 <= i < |parents| :: parents[i], reprUnion(parents)
       requires forall parent :: parent in parents ==> parent.Valid()
     {
-      var visitMap := (x: TreeNode) reads x => rightStackVisited(x, visited);
-      stack == Seq.Flatten(Seq.Map(visitMap, parents)) || (|parents| > 0 && stack == Seq.Flatten(Seq.Map(visitMap, parents[..|parents|-1]))+childStack(parents[|parents|-1]))
+      stack == allRight(parents, visited) || (|parents| > 0 && stack == allRightPlusChildren(parents, visited))
     }
     
     method {:verify false} {:vcs_split_on_every_assert} Traverse(root: TreeNode) returns (result: seq<TreeNode>)
